pulse/examples/dsls/mini_steel/Pulse.Syntax.Printer.fsti
@@ -1,11 +1,12 @@
 module Pulse.Syntax.Printer
 open Pulse.Syntax
 module R = FStar.Reflection
+module T = FStar.Tactics
 
 val name_to_string (f:R.name) : string
 val constant_to_string (c:constant) : string
 val univ_to_string (u:universe) : string
 val qual_to_string (q:option qualifier) : string
-val binder_to_string (b:binder) : string
-val term_to_string (t:term) : string
-val comp_to_string (c:comp) : string
+val binder_to_string (b:binder) : T.Tac string
+val term_to_string (t:term) : T.Tac string
+val comp_to_string (c:comp) : T.Tac string
